Update irods_v5_api_rfc.v

irods_v5_api_rfc.v
@@ -68,74 +68,64 @@ Parameter el : objects -> Set.
 
 (** We identify objects by their identifiers. [identifier] returns the identifer type of an object. *)
 
-Parameter identifier : objects -> Set.
+Parameter identifier_type : objects -> Set.
 
-(** An object is either mutable or immutable. *)
+Parameter identifier : forall {obj : objects}, el obj -> identifier_type obj.
 
-Parameter mutability : objects -> bool.
-
-(** The identifier of an immutable object is its content. *)
-
-Axiom identifier_of_immutable_object_is_content:
-forall (obj : objects), mutability obj = false -> identifier obj = el obj.
-
-(** A mutable object has an identifier that may be different from its content. *)
+(** The identifier of an object is unique. *)
+Axiom identifier_unique:
+forall (obj : objects) (a b : el obj),
+identifier a = identifier b -> a = b.
 
 (** 
-*** List of Immutable Types
+*** List of Types
 *)
 
-Parameter id : Set.
-Parameter resc_name : Set.
-Parameter data_object_name : Set.
-Parameter file_name : Set.
-Parameter zone_name : Set.
-Parameter user_name : Set.
-Parameter group_name : Set.
-Parameter rule_name : Set.
-Parameter microservice_name : Set.
-Parameter API_name : Set.
-Parameter path : Set.
-Parameter physical_path : Set.
-Parameter offset : Set.
-Parameter length : Set.
-Parameter buffer : Set.
-Parameter chksum : Set.
-Parameter error : Set.
-Parameter replica_content : Set.
-Parameter access : Set.
-Parameter iCAT : Set.
-Parameter host : Set.
-Parameter port : Set.
-Parameter config : Set.
-Parameter AVU : Set.
+Parameter id : objects.
+Parameter resc_name : objects.
+Parameter data_object_name : objects.
+Parameter file_name : objects.
+Parameter zone_name : objects.
+Parameter user_name : objects.
+Parameter group_name : objects.
+Parameter rule_name : objects.
+Parameter microservice_name : objects.
+Parameter API_name : objects.
+Parameter path : objects.
+Parameter physical_path : objects.
+Parameter offset : objects.
+Parameter length : objects.
+Parameter buffer : objects.
+Parameter chksum : objects.
+Parameter error : objects.
+Parameter replica_content : objects.
+Parameter access : objects.
+Parameter iCAT : objects.
+Parameter host : objects.
+Parameter port : objects.
+Parameter config : objects.
+Parameter AVU : objects.
+Parameter data_object : objects.
+Parameter collection : objects.
+Parameter resource : objects.
+Parameter replica : objects.
+Parameter user : objects.
+Parameter group : objects.
+Parameter zone : objects.
+Parameter metadata : objects.
+Parameter rule : objects.
+Parameter microservice : objects.
+Parameter PEP : objects.
+Parameter API : objects.
+Parameter connection : objects.
+Parameter data_object_descriptor : objects.
 
 (** 
-*** Constants of immutable types 
+*** List of Constants
 *)
 
-Parameter empty_content : replica_content.
-Parameter null read write own : access.
-
-
-(** 
-*** List of Mutable Types
-*)
-
-Parameter data_object : Set.
-Parameter collection : Set.
-Parameter resource : Set.
-Parameter replica : Set.
-Parameter user : Set.
-Parameter group : Set.
-Parameter zone : Set.
-Parameter metadata : Set.
-Parameter rule : Set.
-Parameter microservice : Set.
-Parameter PEP : Set.
-Parameter API : Set.
-Parameter connection : Set.
-Parameter data_object_descriptor : Set.
+Parameter empty_content : el replica_content.
+Parameter null read write own : el access.
 
 (** 
 ** Relations
@@ -156,24 +146,24 @@ Parameter is_observed : relation -> observed_state -> Prop.
 *** List of Relations 
 *)
 
-Parameter data_object_child_of_collection : data_object -> collection -> relation.
-Parameter collection_child_of_collection : collection -> collection -> relation.
-Parameter collection_root : collection -> relation.
-Parameter replica_of : replica -> data_object -> relation.
-Parameter stored_at : replica -> resource -> relation.
-Parameter resource_child_of_resource : resource -> resource -> relation.
-Parameter resource_root : resource -> relation.
-Parameter resource_local_to_zone : resource -> zone -> relation.
-Parameter replica_local_to_zone : user -> zone -> relation.
-Parameter user_has_access_to_data_object : user -> access -> data_object -> relation.
-Parameter user_has_access_to_collection : user -> access -> collection -> relation.
-Parameter data_object_has_owner: data_object -> user -> relation.
-Parameter path_of_data_object : path -> data_object -> relation.
-Parameter id_of_data_object : id -> data_object -> relation.
-Parameter owner_of_data_object : user -> data_object -> relation.
-Parameter content_of_replica : replica_content -> replica -> relation.
-Parameter path_of_collection : path -> collection -> relation.
-Parameter id_of_collection : id -> collection -> relation.
+Parameter data_object_child_of_collection : el data_object -> el collection -> relation.
+Parameter collection_child_of_collection : el collection -> el collection -> relation.
+Parameter collection_root : el collection -> relation.
+Parameter replica_of : el replica -> el data_object -> relation.
+Parameter stored_at : el replica -> el resource -> relation.
+Parameter resource_child_of_resource : el resource -> el resource -> relation.
+Parameter resource_root : el resource -> relation.
+Parameter resource_local_to_zone : el resource -> el zone -> relation.
+Parameter replica_local_to_zone : el user -> el zone -> relation.
+Parameter user_has_access_to_data_object : el user -> el access -> el data_object -> relation.
+Parameter user_has_access_to_collection : el user -> el access -> el collection -> relation.
+Parameter data_object_has_owner: el data_object -> el user -> relation.
+Parameter path_of_data_object : el path -> el data_object -> relation.
+Parameter id_of_data_object : el id -> el data_object -> relation.
+Parameter owner_of_data_object : el user -> el data_object -> relation.
+Parameter content_of_replica : el replica_content -> el replica -> relation.
+Parameter path_of_collection : el path -> el collection -> relation.
+Parameter id_of_collection : el id -> el collection -> relation.
 
 (** 
 ** Constraints 
@@ -185,16 +175,16 @@ The types and relations must conform to certain constraints.
 *)
 
 Axiom data_object_is_child_of_a_collection:
-forall (s : observed_state) (a : data_object), 
-exists (b : collection), is_observed (data_object_child_of_collection a b) s.
+forall (s : observed_state) (a : el data_object), 
+exists (b : el collection), is_observed (data_object_child_of_collection a b) s.
 
 Axiom data_object_has_at_least_one_replica:
-forall (s : observed_state) (a : data_object), 
-exists (b : replica), is_observed (replica_of b a) s.
+forall (s : observed_state) (a : el data_object), 
+exists (b : el replica), is_observed (replica_of b a) s.
 
 Axiom collection_is_child_of_a_collection_or_root:
-forall (s : observed_state) (a : collection), 
-exists (b : collection), is_observed (collection_child_of_collection a b) s \/ is_observed (collection_root a) s.
+forall (s : observed_state) (a : el collection), 
+exists (b : el collection), is_observed (collection_child_of_collection a b) s \/ is_observed (collection_root a) s.
 
 (**
 * iRODS Interaction Model
@@ -204,7 +194,7 @@ iRODS interaction model defines the dynamic aspect of iRODS.
 There are three type of interactions: actions, queries, and auxiliary functions.
 *)
 
-Parameter action : Set -> Set.
+Parameter action : Set -> Type.
 Parameter query : Set -> Set.
 Parameter aux : Set -> Set.
 
@@ -214,7 +204,7 @@ Parameter aux : Set -> Set.
 Actions can be applied. An applied action has the following type 
 *)
 
-Definition applied_action a := system_state -> (a + error) * system_state.
+Definition applied_action a := system_state -> (a + el error) * system_state.
 
 Parameter apply_action : forall {a : Set}, action a -> applied_action a.
 
@@ -226,27 +216,27 @@ An applied action produces a result [a], can modify the system_state, and can th
 
 Parameter set : relation -> action unit.
 Parameter reset : relation -> action unit.
-Parameter new_id : action id.
-Parameter new_data_object : action data_object.
-Parameter new_replica : resource -> path -> action replica.
-Parameter data_object_copy : data_object -> path -> connection -> action unit.
-Parameter data_object_chksum : data_object -> connection -> action chksum.
-Parameter data_object_rename : data_object -> path -> connection -> action unit.
-Parameter data_object_phymv : data_object -> physical_path -> connection -> action unit.
-Parameter data_object_lock : data_object -> connection -> action unit.
-Parameter data_object_unlock : data_object -> connection -> action unit.
-Parameter data_object_create : resource -> path -> connection -> action unit.
-Parameter data_object_delete : data_object -> connection -> action unit.
-Parameter data_object_unlink : data_object -> path -> connection -> action unit.
-Parameter data_object_open : data_object -> connection -> action data_object_descriptor.
-Parameter data_object_lseek : data_object_descriptor -> offset -> connection -> action unit.
-Parameter data_object_close : data_object_descriptor -> connection -> action unit.
-Parameter data_object_read : data_object_descriptor -> offset -> length -> connection -> action buffer.
-Parameter data_object_write : data_object_descriptor -> offset -> buffer -> connection -> action unit.
-Parameter data_object_replicate : user -> data_object -> resource -> connection -> action unit.
-Parameter data_object_trim : data_object -> resource -> connection -> action unit.
-Parameter data_object_truncate : data_object -> length -> connection -> action unit.
-Parameter data_object_rsync : data_object -> data_object -> connection -> action unit.
+Parameter new_id : action (el id).
+Parameter new_data_object : action (el data_object).
+Parameter new_replica : el resource -> el path -> action (el replica).
+Parameter data_object_copy : el data_object -> el path -> el connection -> action unit.
+Parameter data_object_chksum : el data_object -> el connection -> action (el chksum).
+Parameter data_object_rename : el data_object -> el path -> el connection -> action unit.
+Parameter data_object_phymv : el data_object -> el physical_path -> el connection -> action unit.
+Parameter data_object_lock : el data_object -> el connection -> action unit.
+Parameter data_object_unlock : el data_object -> el connection -> action unit.
+Parameter data_object_create : el resource -> el path -> el connection -> action unit.
+Parameter data_object_delete : el data_object -> el connection -> action unit.
+Parameter data_object_unlink : el data_object -> el path -> el connection -> action unit.
+Parameter data_object_open : el data_object -> el connection -> action (el data_object_descriptor).
+Parameter data_object_lseek : el data_object_descriptor -> el offset -> el connection -> action unit.
+Parameter data_object_close : el data_object_descriptor -> el connection -> action unit.
+Parameter data_object_read : el data_object_descriptor -> el offset -> el length -> el connection -> action (el buffer).
+Parameter data_object_write : el data_object_descriptor -> el offset -> el buffer -> el connection -> action unit.
+Parameter data_object_replicate : el user -> el data_object -> el resource -> el connection -> action unit.
+Parameter data_object_trim : el data_object -> el resource -> el connection -> action unit.
+Parameter data_object_truncate : el data_object -> el length -> el connection -> action unit.
+Parameter data_object_rsync : el data_object -> el data_object -> el connection -> action unit.
 Parameter data_object_get : action unit.
 Parameter data_object_put : action unit.
 
@@ -269,9 +259,9 @@ forall (s : system_state) (a : Set) (qu : query a), snd (apply_action (lift_quer
 *** List of Queries 
 *)
 
-Parameter path_to_data_object : path -> query data_object.
-Parameter path_to_collection : path -> query collection.
-Parameter connection_user : connection -> query user.
+Parameter path_to_data_object : el path -> query (el data_object).
+Parameter path_to_collection : el path -> query (el collection).
+Parameter connection_user : el connection -> query (el user).
 
 (** 
 ** Auxiliary Functions 
@@ -298,7 +288,7 @@ forall (s1 s2 : system_state) (a : Set) (qu : query a), fst (apply_action (lift_
 *** List of Auxiliary Functions 
 *)
 
-Parameter parent_path : path -> aux path.
+Parameter parent_path : el path -> aux (el path).
 
 (** 
 ** DAGs of Actions
@@ -308,6 +298,7 @@ Complex actions can be composed as DAG of actions. The following combinators fro
 
 Parameter pure : forall {a : Set}, a -> action a.
 Parameter bind : forall {a b : Set}, (a -> action b) -> action a -> action b.
+Parameter zero : forall {a : Set}, action a.
 Parameter plus : forall {a : Set}, action a -> action a -> action a.
 
 (**
@@ -315,12 +306,6 @@ Parameter plus : forall {a : Set}, action a -> action a -> action a.
 The interaction model needs to satisfy the follow constraints.
 *)
 
-Axiom id_of_data_object_immutability:
-forall (s s' : system_state) (a : Set) (act : action a),
-snd (apply_action act s) = s' -> 
-forall (i : id) (a b : data_object), 
-is_system (id_of_data_object i a) s /\ is_system (id_of_data_object i b) s' ->
-a = b.
 
 End iRODS_model.
 
@@ -336,217 +321,247 @@ Parameter byte_array : Set.
 Parameter empty_byte_array : byte_array.
 End data_types.
 
-Module iRODS_data_impl (dt : data_types) <: iRODS_model.
+Module iRODS_model_impl (dt : data_types) <: iRODS_model.
 
 Import dt.
 
+Definition system_state := unit.
+Definition observed_state := unit.
+Definition observe (s : system_state) : observed_state := s.
 (** 
-*** Immutable Sets 
+*** Type Names
 *)
 
-Inductive immutable_objects := 
-  | id_object : immutable_objects
-  | resc_name_object : immutable_objects
-  | data_object_name_object : immutable_objects
-  | file_name_object : immutable_objects
-  | zone_name_object : immutable_objects
-  | user_name_object : immutable_objects
-  | group_name_object : immutable_objects
-  | rule_name_object : immutable_objects
-  | microservice_name_object : immutable_objects
-  | API_name_object : immutable_objects
-  | path_object : immutable_objects
-  | physical_path_object : immutable_objects
-  | offset_object : immutable_objects
-  | length_object : immutable_objects
-  | buffer_object : immutable_objects
-  | chksum_object : immutable_objects
-  | error_object : immutable_objects
-  | replica_content_object : immutable_objects
-  | access_object : immutable_objects
-  | iCAT_object : immutable_objects
-  | host_object : immutable_objects
-  | port_object : immutable_objects
-  | config_object : immutable_objects
-  | AVU_object : immutable_objects.
+Inductive _objects := 
+  | _id
+  | _resc_name
+  | _data_object_name
+  | _file_name
+  | _zone_name
+  | _user_name
+  | _group_name
+  | _rule_name
+  | _microservice_name
+  | _API_name
+  | _path
+  | _physical_path
+  | _offset
+  | _length
+  | _buffer
+  | _chksum
+  | _error
+  | _replica_content
+  | _access
+  | _iCAT
+  | _host
+  | _port
+  | _config
+  | _AVU
+  | _data_object
+  | _collection
+  | _resource
+  | _replica
+  | _user
+  | _group
+  | _zone
+  | _metadata
+  | _rule
+  | _microservice
+  | _PEP
+  | _API
+  | _connection
+  | _data_object_descriptor.
+  
+  
+Definition objects := _objects.
+Definition id := _id.
+Definition resc_name := _resc_name.
+Definition data_object_name := _data_object_name.
+Definition file_name := _file_name.
+Definition zone_name := _zone_name.
+Definition user_name := _user_name.
+Definition group_name := _group_name.
+Definition rule_name := _rule_name.
+Definition microservice_name := _microservice_name.
+Definition API_name := _API_name.
+Definition path := _path.
+Definition physical_path := _physical_path.
+Definition offset := _offset.
+Definition length := _length.
+Definition buffer := _buffer.
+Definition chksum := _chksum.
+Definition error := _error.
+Definition replica_content := _replica.
+Definition access := _access.
+Definition iCAT := _iCAT.
+Definition host := _host.
+Definition port := _port.
+Definition config := _config.
+Definition AVU := _AVU.
+Definition data_object := _data_object.
+Definition collection := _collection.
+Definition resource := _resource.
+Definition replica := _replica.
+Definition user := _user.
+Definition group := _group.
+Definition zone := _zone.
+Definition metadata := _metadata.
+Definition rule := _rule.
+Definition microservice := _microservice.
+Definition PEP := _PEP.
+Definition API := _API.
+Definition connection := _collection.
+Definition data_object_descriptor := _data_object_descriptor.
 
-(** 
-*** Mutable Sets 
-*)
+Inductive access_type := null | read | write | own.
 
-Inductive mutable_objects :=
-  | data_object_object : mutable_objects
-  | collection_object : mutable_objects
-  | resource_object : mutable_objects
-  | replica_object : mutable_objects
-  | user_object : mutable_objects
-  | group_object : mutable_objects
-  | zone_object : mutable_objects
-  | metadata_object : mutable_objects
-  | rule_object : mutable_objects
-  | microservice_object : mutable_objects
-  | PEP_object : mutable_objects
-  | API_object : mutable_objects
-  | connection_object : mutable_objects
-  | data_object_descriptor_object : mutable_objects.
+Definition identifier_type (obj : objects) : Set :=
+  match obj with
+  | _id => integer
+  | _resc_name => string
+  | _data_object_name => string
+  | _file_name => string
+  | _zone_name => string
+  | _user_name => string
+  | _group_name => string
+  | _rule_name => string
+  | _microservice_name => string
+  | _API_name => string
+  | _path => string
+  | _physical_path => string
+  | _offset => integer
+  | _length => integer
+  | _buffer => byte_array
+  | _chksum => string
+  | _error => integer * string
+  | _replica_content => byte_array
+  | _access => access_type
+  | _iCAT => string
+  | _host => string
+  | _port => integer
+  | _config => tree
+  | _AVU => string * string * string
+(** A data object is identified by a zone and an integer. *)
 
+  | _data_object => string * integer
+(** A collection is identified by a zone and an integer. *)
 
-Definition id := integer.
-Definition resc_name := string.
-Definition data_object_name := string.
-Definition file_name := string.
-Definition zone_name := string.
-Definition user_name := string.
-Definition group_name := string.
-Definition rule_name := string.
-Definition microservice_name := string.
-Definition API_name := string.
-Definition path := string.
-Definition physical_path := string.
-Definition offset := integer.
-Definition length := integer.
-Definition buffer := byte_array.
-Definition chksum := string.
-Definition error : Set := integer * string.
-Definition replica_content := byte_array.
-Inductive access := null | read | write | own.
-Definition iCAT := string.
-Definition host := string.
-Definition port := integer.
-Definition config := tree.
-Definition AVU : Set := string * string * string.
+  | _collection => string * integer
+(** A resource is identified by a zone and an integer. *)
 
-Definition empty_content := empty_byte_array.
+  | _resource => string * integer
 
-Definition data_object : Set := zone_name * id.
-Definition collection : Set := zone_name * id.
-Definition resource : Set := zone_name * id.
+(** A replica is identified by a zone, a resource, and a path on that resource. *)
 
-(** Replica is identified by a zone, a resource, and a path on that resource. *)
+  | _replica => string * integer * string
 
-Definition replica : Set := zone_name * id * physical_path.
+(** A user or group is identified by a zone and a user name in that zone. *)
 
-(** User or group is identified by a zone and a user name in that zone. *)
-
-Definition user : Set := zone_name * user_name.
-Definition group : Set := zone_name * user_name.
-Definition zone := zone_name.
+  | _user => string * string
+  | _group => string * string
+  | _zone => string
 
 (** Metadata is identified by AVU. *)
 
-Definition metadata := AVU.
-Definition rule : Set := host * rule_name.
-Definition microservice : Set := host * microservice_name.
-Definition PEP : Set := host * rule_name.
-Definition API : Set := host * id.
-Definition connection : Set := host * id.
-Definition data_object_descriptor : Set := host * id.
+  | _metadata => string * string * string
+  
+(** A rule is identified by a host and a rule name *)
 
-Definition objects : Set := immutable_objects + mutable_objects.
+  | _rule => string * string
+(** A microservice is identified by a host and a microservice name *)
 
-Definition el (o : objects) : Set :=
-  match o with
-  | inl io => match io with
-    | id_object => id
-    | resc_name_object => resc_name
-    | data_object_name_object => data_object_name
-    | file_name_object => file_name
-    | zone_name_object => zone_name
-    | user_name_object => user_name
-    | group_name_object => group_name
-    | rule_name_object => rule_name
-    | microservice_name_object => microservice_name
-    | API_name_object => API_name
-    | path_object => path
-    | physical_path_object => physical_path
-    | offset_object => offset
-    | length_object => length
-    | buffer_object => buffer
-    | chksum_object => chksum
-    | error_object => error
-    | replica_content_object => replica_content
-    | access_object => access
-    | iCAT_object => iCAT
-    | host_object => host
-    | port_object => port
-    | config_object => config
-    | AVU_object => AVU
-    end
-  | inr mo =>
-    match mo with
-      | data_object_object => data_object
-      | collection_object => collection
-      | resource_object => resource
-      | replica_object => replica
-      | user_object => user
-      | group_object => group
-      | zone_object => zone
-      | metadata_object => metadata
-      | rule_object => rule
-      | microservice_object => microservice
-      | PEP_object => PEP
-      | API_object => API
-      | connection_object => connection
-      | data_object_descriptor_object => data_object_descriptor
-    end
+  | _microservice => string * string
+
+(** A PEP is identified by a host and a PEP name *)
+
+  | _PEP => string * string
+(** An API is identified by a host and an API id *)
+
+  | _API => string * integer
+(** A connection is identified by a host and a connection id *)
+
+  | _connection => string * integer
+(** A data_object_descriptor is identified by a host and a data_object_descriptor id *)
+
+  | _data_object_descriptor => string * integer
   end.
 
 
+Definition empty_content := empty_byte_array.
+
 (** We identify the identifier of an object with the object. *)
 
-Definition identifier := el.
+Definition el := identifier_type.
 
-Parameter relation : Set.
+Definition identifier {obj : objects} (x : el obj) : identifier_type obj := x.
 
-Parameter data_object_child_of_collection : data_object -> collection -> relation.
-Parameter collection_child_of_collection : collection -> collection -> relation.
-Parameter collection_root : collection -> relation.
-Parameter replica_of : replica -> data_object -> relation.
-Parameter stored_at : replica -> resource -> relation.
-Parameter resource_child_of_resource : resource -> resource -> relation.
-Parameter resource_root : resource -> relation.
-Parameter resource_local_to_zone : resource -> zone -> relation.
-Parameter replica_local_to_zone : user -> zone -> relation.
-Parameter user_has_access_to_data_object : user -> access -> data_object -> relation.
-Parameter user_has_access_to_collection : user -> access -> collection -> relation.
-Parameter data_object_has_owner: data_object -> user -> relation.
-Parameter path_of_data_object : path -> data_object -> relation.
-Parameter id_of_data_object : id -> data_object -> relation.
-Parameter owner_of_data_object : user -> data_object -> relation.
-Parameter content_of_replica : replica_content -> replica -> relation.
-Parameter path_of_collection : path -> collection -> relation.
-Parameter id_of_collection : id -> collection -> relation.
+Lemma identifier_unique : 
+forall (obj : objects) (a b : el obj),
+identifier a = identifier b -> a = b.
+Proof.
+unfold identifier. auto.
+Qed.
+
+Inductive _relation : Set :=
+  | data_object_child_of_collection : el data_object -> el collection -> _relation
+  | collection_child_of_collection : el collection -> el collection -> _relation
+  | collection_root : el collection -> _relation
+  | replica_of : el replica -> el data_object -> _relation
+  | stored_at : el replica -> el resource -> _relation
+  | resource_child_of_resource : el resource -> el resource -> _relation
+  | resource_root : el resource -> _relation
+  | resource_local_to_zone : el resource -> el zone -> _relation
+  | replica_local_to_zone : el user -> el zone -> _relation
+  | user_has_access_to_data_object : el user -> el access -> el data_object -> _relation
+  | user_has_access_to_collection : el user -> el access -> el collection -> _relation
+  | data_object_has_owner: el data_object -> el user -> _relation
+  | path_of_data_object : el path -> el data_object -> _relation
+  | id_of_data_object : el id -> el data_object -> _relation
+  | owner_of_data_object : el user -> el data_object -> _relation
+  | content_of_replica : el replica_content -> el replica -> _relation
+  | path_of_collection : el path -> el collection -> _relation
+  | id_of_collection : el id -> el collection -> _relation.
+  
+Definition relation := _relation.
+
+(** *** Queries *)
+
+Inductive _query : Set -> Set :=
+  | path_to_data_object : el path -> _query (el data_object)
+  | path_to_collection : el path -> _query (el collection)
+  | connection_user : el connection -> _query (el user).
+  
+Definition query := _query.
+
+(** *** Auxiliary Functions *)
+
+Inductive _aux : Set -> Set :=
+  | parent_path : el path -> _aux (el path).
+  
+Definition aux := _aux.
 
 (** *** Actions *)
 
-Parameter action : Set -> Set.
-Parameter pure : forall {a : Set}, a -> action a.
-Parameter bind : forall {a b : Set}, (a -> action b) -> action a -> action b.
-Parameter plus : forall {a : Set}, action a -> action a -> action a.
-Parameter set : relation -> action unit.
-Parameter reset : relation -> action unit.
-Parameter new_id : action id.
-Parameter new_data_object : action data_object.
-Parameter new_replica : resource -> path -> action replica.
+Inductive _action : Set -> Type :=
+  | pure : forall {a : Set}, a -> _action a
+  | bind : forall {a b : Set}, (a -> _action b) -> _action a -> _action b
+  | plus : forall {a : Set}, _action a -> _action a -> _action a
+  | set : relation -> _action unit
+  | reset : relation -> _action unit
+  | new_id : _action (el id)
+  | new_data_object : _action (el data_object)
+  | new_replica : el resource -> el path -> _action (el replica)
+  | lift_query : forall {a : Set}, query a -> _action a
+  | lift_aux : forall {a : Set}, aux a -> _action a.
+  
+Definition action := _action.
 
 (** MonadPlus notations *)
 
 Notation "a >>= b" := (bind b a) (at level 10).
 Notation "a | b" := (plus a b) (at level 11).
 
-(** *** Queries *)
 
-Parameter query : Set -> Set.
-Parameter lift_query : forall {a : Set}, query a -> action a.
-Parameter path_to_data_object : path -> query data_object.
-Parameter path_to_collection : path -> query collection.
-Parameter connection_user : connection -> query user.
-
-(** *** Auxiliary Functions *)
-
-Parameter aux : Set -> Set.
-Parameter lift_aux : forall {a : Set}, aux a -> action a.
-Parameter parent_path : path -> aux path.
 
 (** *** List of Actions *)
 (** Some auxiliary definitions *)
@@ -563,7 +578,7 @@ Definition lift_query1 {a b: Set} (q1 : a -> query b) (acta : action a) : action
 
 (** *** Data Object Create *)
 
-Definition data_object_create (r : resource) (p : path) (c : connection) :=
+Definition data_object_create (r : el resource) (p : el path) (c : el connection) :=
   let u := lift_query (connection_user c) in
   let di := new_id in
   let d := new_data_object in
